haskell/Optics2/src/Traversal.hs
@@ -1,0 +1,14 @@
+module  Traversal
+    (   ex1, ex2, ex3
+    )   where
+
+import Control.Lens
+
+ex1 :: [String]
+ex1 = ("Bubbles","Buttercup") ^.. both
+
+ex2 :: (String, String)
+ex2 = over both (++ "!") ("Bubbles","Buttercup")
+
+ex3 :: (String, String)
+ex3 = ("Bubbles","Buttercup") & both %~ (++ "!")
