coq/logic/Composition.v
@@ -6,4 +6,6 @@ Definition comp (v w u:Type) (g:w -> u) (f:v -> w) (x:v) : u := g (f x).
 Arguments comp {v} {w} {u} _ _ _.
 
 Notation "g ; f" := (comp g f) 
-    (at level 60, right associativity) : Composition.
+    (at level 60, right associativity) : Composition_scope.
+
+Open Scope Composition_scope.
