coq/logic/In.v
@@ -1,0 +1,5 @@
+Require Import List.
+
+Notation "x :: xs" := (In x xs) : In_scope.
+
+Open Scope In_scope.
