lean/WellFounded.lean
@@ -265,3 +265,15 @@ def AccessibleInv : ∀ {α : Type u} (r : α → α → Prop) (x : α),
             | ⟨_,q⟩ := q
             end
 
+#check @well_founded.fix -- counterpart of Fix in Coq
+
+/-
+def WFRecursion_F : ∀ {α : Type u} (r : α → α → Prop) (c : α → Type u),
+  (∀ (x:α), (∀ (y:α), r y x → c y) → c x) →
+   ∀ (x:α), Accessible r x → c x :=
+     λ (α:Type u),
+       λ (r:α → α → Prop),
+         λ (c:α → Type u),
+           λ (IH:∀ (x:α), (∀(y:α), r y x → c y) → c x),
+-/
+
